\documentclass{beamer}
\usetheme{CambridgeUS}
\usepackage{csquotes}
\usepackage{comment}
\usepackage{amsmath,amssymb,amsthm}
\usepackage{enumerate}
\usepackage{graphicx}
\title{Assignment 5}
     \author{PUNDI BINDUSREE \\
     CS21BTECH11048 \\
     Papoulis Chapter6 Ex-6.25\\ }
     \date{\today}
\logo{\large \LaTeX{}}  

\begin{document}
     
\begin{frame}
    \maketitle    
\end{frame}
     
     \logo{}
     
     \begin{frame}{Outline}
    \tableofcontents
     \end{frame}


\section{Question}
\begin{frame}{Question}
\begin{block}{Question}
Let \textbf{x} be the lifetime of a certain electric bulb, and y that of its replacement after the failure of the first bulb. Suppose \textbf{x} and \textbf{y} are independent with common exponential density function with parameter $\lambda$.Find the probability that the combined lifetime exceeds 2$\lambda$. What is the probability that the replacement outlasts the original component by $\lambda$?
\end{block}
\end{frame}


\section{Solution}
\begin{frame}{solution}
Given\\
\begin{itemize}
    \item the lifetime of a certain electric bulb = \textbf{x}
    \item and lifetime of its replacement after the failure of the first bulb = \textbf{y}
    \item and also given that \textbf{x} and \textbf{y} are independent with common exponential density function with parameter $\lambda$ .
\end{itemize}
\end{frame}


\begin{frame}{solution}
\begin{itemize}
    \item pdf of an exponential distribution of X with parameter $\lambda$ = $\frac{1}{\lambda}e^{-\frac{x}{\lambda}}u(x)$
    \item pdf of an exponential distribution of Y with parameter $\lambda$ = $\frac{1}{\lambda}e^{-\frac{y}{\lambda}}u(y)$
\end{itemize}
\end{frame}
     
     
\begin{frame}{solution}
Given that X and Y are independent therefore
\begin{enumerate}
    \item $f_{XY}(x,y) = f_{X}(x).f_{Y}(y)$
    \item Let Z=X+Y
\end{enumerate}
\end{frame}


\begin{frame}{solution}
\begin{enumerate}
\setcounter{enumi}{2}

\item 
\begin{align}
    \text{then }f_{Z}(z) & = \int_{x=0}^{z}f_{XY}(x,y)dx.dy{      z>0}\\
                         & = \int_{x=0}^{z}f_{X}(x)f_{Y}(y)dxdy\\
                         & = \int_{x=0}^{z}f_{X}(x)f_{Y}(z-x)dx
\end{align}
\end{enumerate}
\end{frame}


\begin{frame}{solution}
\begin{align}
                         & = \int_{x=0}^{z}({\frac{1}{\lambda}})^2e^{-\frac{x}{\lambda}}e^{-\frac{z-x}{\lambda}}dx\\ 
                         & = {\frac{1}{\lambda}}^2\int_{x=0}^{z}e^{-\frac{z}{\lambda}}\int_{x=0}^{z}dx\\
                         & = {\frac{z}{{\lambda}^2}}e^{-\frac{z}{\lambda}}
\end{align}

\end{frame}
     
     
\begin{frame}{solution}
Required to find the probability that the combined lifetime exceeds 2$\lambda$
\begin{enumerate}
\setcounter{enumi}{3}
\item so here Z $>$ 2$\lambda$
\begin{align}
     P(Z>2\lambda) & = \int_{2\lambda}^{\infty}{\frac{z}{{\lambda}^2}}e^{-\frac{z}{\lambda}}dz\\
                   & = \int_{2}^{\infty}ae^{-a}da\\
                   & = 3e^{-2}
    \end{align}
    \end{enumerate}
    \end{frame}
    
    
\begin{frame}{solution}
    \begin{itemize}
       \item so the required probability is $3e^{-2}=0.407$ (approximately by rounding off)
    \end{itemize}   
\end{frame}


\begin{frame}{solution}
\begin{enumerate}
\setcounter{enumi}{4}
\item Now need to find the probability that the replacement outlasts the original component by $\lambda$
\begin{itemize}
    \item Let W=Y-X
    \item then Y=W+X
    \end{itemize}
    \end{enumerate}
    \end{frame}
    
    
\begin{frame}{solution}
    \begin{enumerate}
        \item  similarly from above process we get the required probability as
        \begin{itemize}
       \item
    \begin{align}
     f_{W}(w) & = \int_{x=0}^{z}f_{X}(x)f_{Y}(w+2x)dx\\
              & = \int_{x=0}^{z}({\frac{1}{\lambda}})^2e^{-\frac{x}{\lambda}}e^{-\frac{w+2x}{\lambda}}dx\\ 
              & = \frac{1}{2\lambda}e^{-\frac{w}{\lambda}},{   w>0}
    \end{align}
\end{itemize}
\end{enumerate}
\end{frame}


\begin{frame}{solution}
\begin{enumerate}
\setcounter{enumi}{5}
\item now here $w>\lambda$ 
\begin{align}
F_{W}(w) & = \int_{\lambda}^{\infty}\frac{1}{2\lambda}e^{-\frac{w}{\lambda}}dw\\
         & = \frac{1}{2e}
\end{align}

\end{enumerate}
\end{frame}


\begin{frame}{solution}
\begin{itemize}
    \item Therefore the required probability that replacement outlasts the original component by $\lambda$ is = $\frac{1}{2e}$
\end{itemize}
\end{frame}

\end{document}
